# 正誤表
## 1刷〜
| &nbsp;&nbsp;&nbsp;&nbsp;&nbsp;&nbsp;&nbsp;&nbsp;&nbsp;&nbsp;&nbsp;&nbsp;&nbsp; <br>ページ<br>&nbsp; |&nbsp;&nbsp;&nbsp;&nbsp;&nbsp;&nbsp;&nbsp;&nbsp;&nbsp;&nbsp;&nbsp;&nbsp;&nbsp;&nbsp;&nbsp;&nbsp;&nbsp;&nbsp;&nbsp;&nbsp;&nbsp;&nbsp;&nbsp;&nbsp;&nbsp;&nbsp;&nbsp; <br>場所<br>&nbsp; |  &nbsp;<br>誤<br>&nbsp;  |  &nbsp;<br>正<br>&nbsp;  | &nbsp;&nbsp;&nbsp;&nbsp;&nbsp;&nbsp;&nbsp;&nbsp;&nbsp; <br>備考<br>&nbsp;&nbsp;&nbsp;&nbsp;&nbsp;&nbsp; |
| :---: | :------: | ---- | ---- | ---- |
|p.135|定理4.5<br>第二移動定理|$\mathcal{L}^{-1} \\{\mathcal{U}(t-a)f(t-a)\\} = e^{-as}F(s)$|$\mathcal{L}\\{\mathcal{U}(t-a)f(t-a)\\} = e^{-as}F(s)$||
|p.139|問題4.1|$\left.-\dfrac{e^{-(s-a)^{t}}}{s-a}\right\\|^\infty_0$|$\left.-\dfrac{e^{-(s-a)t}}{s-a}\right\\|^\infty_0$||
|p.156|問題4.40<br>別解| (1)式に $s$ をかけて $A$ を求め， $s\rightarrow\infty$ とすると， $A+B=0$ または $B=-A=-2$ となり， $A+B=0$ または $B=-A=-2$ が得られる．|$A$ を求めたあと，(1)に $s$ をかけて $s\rightarrow\infty$ とすると， $A+B=0$ または $B=-2$ が得られる。||
|p.156|問題4.41<br>別解|(1)式に $s$ をかけて $A$ を求め， $s\rightarrow\infty$ とすると， $A+D=0$ または $D=1$ が得られ，より簡単に結果が得られる．|$A$ を求めたあと，(1)式に $s$ をかけて， $s\rightarrow\infty$ とすると， $A+D=0$ または $D=1$ が得られ，より簡単に結果が得られる．||
